---
{"dg-publish":true,"permalink":"/1-2-1-exercises/","created":"","updated":""}
---


>[!exmp] Example (1)
> Let us start considering the constant function $f(x)=c$ with $x\in\mathbb{R}$, and prove that 
> $$ 
> \lim_{x\rightarrow x_{0}} f(x)= f(x_{0}).
> $$ 
> Indeed, it immediately follows that $|f(x) - f(x_{0})|=0<\epsilon$ for every $x\in\mathbb{R}$ and every $\epsilon>0$.
> 
> Now, let us consider the function $f(x)=x$, and prove that 
> $$ 
> \lim_{x\rightarrow x_{0}} f(x)= f(x_{0}).
> $$ 
> Again, it is immediate to check that $|f(x) - f(x_{0})|=|x - x_{0}|$, and thus, taking $\delta_{\epsilon}< \epsilon$, we get that $|x - x_{0}|<\delta_{\epsilon}$ implies $|f(x) - f(x_{0})|<\epsilon$.
> 
> Finally, let us consider the function $f(x)=x^{2}$, and prove that
> $$ 
> \lim_{x\rightarrow x_{0}} f(x)= f(x_{0})
> $$
> for every $x_{0}\in\mathbb{R}$.  We have
> $$
> |x^{2} - x_{0}^{2}| =|(x+x_{0})(x-x_{0})|\leq (|x| + |x_{0}|)|x-x_{0}| .
> $$
> Recall that we must check that $|f(x) - f(x_{0})|< \epsilon$ whenever $|x - x_{0}|<\delta$, with $\delta>0$ to be determined depending on $\epsilon>0$.  A direct computation shows that 
> $$
> | x+ x_{0}| =|x - x_{0} + 2x_{0}|\leq |x - x_{0}| + 2|x_{0}|
> $$ 
> so that
> $$
> |x^{2} - x_{0}^{2}|\leq (|x - x_{0}| + 2|x_{0}|)\,|x-x_{0}| < (2|x_{0}| + \delta_{\epsilon})\,\delta_{\epsilon}.
>$$
>Therefore, if 
>$$
>\delta_{\epsilon}^{2} + 2|x_{0}| \delta_{\epsilon} - \epsilon>0
>$$
>we are done. By solving the previous [quadratic equation](https://en.wikipedia.org/wiki/Quadratic_equation) in the variable $\delta_{\epsilon}$ we obtain the condition
>$$
> 0 < \delta_{\epsilon} <  \sqrt{x^{2}_{0} + \epsilon} -|x_{0}| = \sqrt{x^{2}_{0} + \epsilon} - \sqrt{x^{2}_{0}}.
>$$
>
