---
{"dg-publish":true,"permalink":"/1-7-exercises/","created":"2023-07-02T17:05:44.464+02:00","updated":"2023-08-30T13:01:28.742+02:00"}
---

# 1 Limits of scalar functions



1) Compute 
	$$ \lim_{x\rightarrow x_{0}} f(x)= f(x_{0}) $$
	for $f(x)=c$, $f(x)=x$, and $f(x)=x^{2}$.  
	>[!note]- Solution 
	>Let us start considering the constant function $f(x)=c$ with $x\in\mathbb{R}$, and prove that
	>	$$ \lim_{x\rightarrow x_{0}} f(x)= f(x_{0}). $$ 
	> Indeed, it immediately follows that $|f(x) - f(x_{0})|=0<\epsilon$ for every $x\in\mathbb{R}$ and every $\epsilon>0$.  Now, let us consider the function $f(x)=x$, and prove that $$ \lim_{x\rightarrow x_{0}} f(x)= f(x_{0}). $$ 
	> Again, it is immediate to check that $|f(x) - f(x_{0})|=|x - x_{0}|$, and thus, taking $\delta_{\epsilon}< \epsilon$, we get that $|x - x_{0}|<\delta_{\epsilon}$ implies $|f(x) - f(x_{0})|<\epsilon$ Finally, let us consider the function $f(x)=x^{2}$, and prove that 
	> $$ \lim_{x\rightarrow x_{0}} f(x)= f(x_{0}) $$ 
	> for every $x_{0}\in\mathbb{R}$.  We have 
	> $$ |x^{2} - x_{0}^{2}| =|(x+x_{0})(x-x_{0})|\leq (|x| + |x_{0}|)|x-x_{0}| . $$ 
	> Recall that we must check that $|f(x) - f(x_{0})|< \epsilon$ whenever $|x - x_{0}|<\delta$, with $\delta>0$ to be determined depending on $\epsilon>0$.  A direct computation shows that 
	> $$ | x+ x_{0}| =|x - x_{0} + 2x_{0}|\leq |x - x_{0}| + 2|x_{0}| $$ 
	> so that 
	> $$ |x^{2} - x_{0}^{2}|\leq (|x - x_{0}| + 2|x_{0}|)\,|x-x_{0}| < (2|x_{0}| + \delta_{\epsilon})\,\delta_{\epsilon}. $$
	> Therefore, if 
	> $$ \delta_{\epsilon}^{2} + 2|x_{0}| \delta_{\epsilon} - \epsilon>0 $$ 
	> we are done. By solving the previous [quadratic equation](https://en.wikipedia.org/wiki/Quadratic_equation) in the variable $\delta_{\epsilon}$ we obtain the condition 
	> $$ 0 < \delta_{\epsilon} <  \sqrt{x^{2}_{0} + \epsilon} -|x_{0}| = \sqrt{x^{2}_{0} + \epsilon} - \sqrt{x^{2}_{0}}. $$
    ---
2) Using previous results and [[1.2 Limits of scalar functions#^f50bb0\|algebraic manipulations of limits]], check that 
	$$ \lim_{x\rightarrow x_{0}} f(x)= f(x_{0}) $$ for  
	$$ f(x)=\sum\limits_{k=0}^{n}a_{k} \,x^{k} $$ with $a_{k}\in\mathbb{R}$. 
	---
3)  Use the [[1.2 Limits of scalar functions#Improper limits\|definition]] to check the following limits: 
	$$ \begin{split} 1) \quad & \lim_{x\rightarrow +\infty}\,x^{n}=+\infty \\ & \\ 2) \quad & \lim_{x\rightarrow -\infty}\,x^{2n}=+\infty \\ & \\ 3) \quad & \lim_{x\rightarrow -\infty}\,x^{2n+1}=-\infty \\ & \\ 4) \quad & \lim_{x\rightarrow 0^{\pm}} \;\frac{1}{x^{2n}} =+ \infty \\& \\ 5) \quad & \lim_{x\rightarrow 0^{\pm}} \;\frac{1}{x^{2n+1}} =\pm \infty \\& \\ 	6)   \quad & \lim_{x\rightarrow \pm\infty} \;\frac{1}{x^{n}} =0 \\& \\ \end{split} $$
	>[!note]- Solution 
	>1) We must prove that, for every $K>0$, there is $M>0$ such that $x>M$ implies $f(x)=x^{n}>K$. Taking $M=\sqrt[n]{K}$, we have $f(x)=x^{n}> M^{n}=K$ as requested.
	>2) We must prove that, for every $K>0$, there is $M>0$ such that $x<-M$ implies $f(x)=x^{2n}>K$. Note that, even if $x<0$, it is $f(x)=x^{2n}>0$, so that $f(x)=x^{2n}>M^{2n}$. Taking $M=\sqrt[2n]{K}$, we have $f(x)=x^{2n}>M^{2n}=K$ as requested.
	>3) The proof is analogous to that in 2). 
	>4) For the right limit ($0^{+}$), we must prove that, for every $K>0$, there is $\delta>0$ such that $x<\delta$ implies $f(x)>K$. Taking $\delta=\frac{1}{\sqrt[2n]{K}}$, we have $f(x)=\frac{1}{x^{2n}}>\frac{1}{\delta^{2n}}=K$ as requested. The proof for the left limit is analogous.
	>5) The proof is analogous to that in 4).
	>6) The proof is analogous to that in 4).
	--- 
4) Consider the function $([0,+\infty),\mathbb{R},f,\mathbb{R})$, where $f(x)=x^{\frac{1}{n}}\equiv\sqrt[n]{x}$ with $n>1$: 
	1) prove it is a continuous function;
	2) find its limit at $+\infty$;
	3) what can we say regarding $f(x)=x^{\frac{m}{n}}$? 
	
	>[!note]- Solution 
	>1) We start noting that $([0,+\infty),\mathbb{R},f,\mathbb{R})$ is the [[1.1 Sets and functions#^ac035a\|inverse function]] of $([0,+\infty),\mathbb{R},g,\mathbb{R})$ where $g(y)=y^{n}$.  In exercise 2) above, we proved that $([0,+\infty),\mathbb{R},g,\mathbb{R})$ is continuous. Therefore, [[1.2 Limits of scalar functions#^0478fa\|its inverse is also continuous]]. 
	>2) We note that $1<M<x$ implies $1<\sqrt[n]{M}<\sqrt[n]{x}$, so that $M=K^{n}$ implies $x^{\frac{1}{n}}>K$,  which means that  $$ \lim_{x\rightarrow+\infty}f(x)=+\infty. $$ 
	>3) Once we know $([0,+\infty),\mathbb{R},f,\mathbb{R})$ is continuous, we can use the [[1.2 Limits of scalar functions#^47f720\|algebra of continuous functions]] to conclude $([0,+\infty),\mathbb{R},h,\mathbb{R})$, where $h(x)=x^{\frac{m}{n}}$, is continuous too.
	---
5) Check the following limits: 
	$$ \begin{split} 1) \quad & \lim_{x\rightarrow 1}\,\frac{x}{x+1}=\frac{1}{2}  \\ & \\ 2) \quad &  \lim_{x\rightarrow 0}\, \frac{x}{|x|}=\nexists \\ & \\ 3) \quad &  \lim_{x\rightarrow 0}\, \frac{|x|}{ x }=\nexists \\ & \\ 4) \quad &  \lim_{x\rightarrow 0}\, f(x) =\nexists \quad \mbox{ with } f(x)= \left\{\begin{matrix} 1-x^{2} & \mbox{ if } x<0 \\ x^{3} & \mbox{ if } x\geq 0\end{matrix}\right.  \\ & \\ 5) \quad &  \lim_{x\rightarrow 1^{\pm}}\, \frac{x^{2}-1}{ x^{2} -2x + 1 }= \pm\infty\\ & \\ 6) \quad &  \lim_{x\rightarrow 2^{+}}\, \frac{\sqrt{x^{2} -4}}{x-2} = +\infty \end{split} $$
	>[!note]- Solution
	>1) Use [[1.2 Limits of scalar functions#^f50bb0\|algebraic manipulation of limits]].
	>2) When $x\rightarrow 0^{+}$, it is $\frac{x}{|x|}=1$, while $\frac{x}{|x|}=-1$ when $x\rightarrow 0^{-}$. Consequently, the left and right limits are different, and the limit for $x\rightarrow 0$ does not exist.
	>3) The proof is analogous to that of 2) above. 
	>4) The proof is analogous to that of 2) above.
	>5) When $x=1$, both numerator and denominator vanish, and we get an indeterminate form. However, the fact that both polynomials have a common root ($x=1$) suggests we [factorize them](https://en.wikipedia.org/wiki/Polynomial#Factoring). In particular, we have $x^{2}-1=(x-1)(x+1)$, and $x^{2}-2x +1=(x-1)(x-1)$. Consequently, we have 
	>	$$ \frac{x^{2}-1}{x^{2}-2x+1}=\frac{x+1}{x-1}=1+ \frac{2}{x-1}. $$ 
	>	To check the right limit, we need to show that, for every $K>0$, there is $\delta>0$ such that  $0<x-1<\delta$ implies $|1+\frac{2}{x-1}|>K$. Now, $\frac{2}{x-1}>0$ when $0<x-1<\delta$, so that $1+\frac{2}{x-1}>1+ \frac{2}{\delta}>K$ provided $\delta<\frac{2}{K-1}$. The left limit is found proceeding in analogy.
	>6) Following the reasoning in point 5), we obtain 
	>	$$ \frac{\sqrt{x^{2}-4}}{x-2}=\sqrt{1+\frac{4}{x-2}}.$$ 		Then, to check the right limit, we need to show that, for every $K>0$, there is $\delta>0$ such that  $0<x-2<\delta$ implies $\sqrt{1+\frac{4}{x-2}}>K$. Now, $\frac{4}{x-2}>0$ when $0<x-2<\delta$, so that $1+\frac{4}{x-2}>1+ \frac{4}{\delta}>K^{2}$ provided $\delta<\frac{4}{K^{2}-1}$.




# 2 Derivatives 



1) Find the derivative of  $f(x)=x^{3}$ and $f(x)=x^{4}$ for every $x_{0}\in\mathbb{R}$. Use  [Newton's binomial formula](https://en.wikipedia.org/wiki/Binomial_theorem)
$$
(a+b)^{n}=\sum\limits_{k=0}^{n}{n\choose k} a^{n-k}b^{k}=\sum\limits_{k=0}^{n}{n\choose k} a^{k}b^{n-k},
$$
where ${n\choose k}=\frac{n!}{k!(n-k)!}$ is the [binomial coefficient](https://en.wikipedia.org/wiki/Binomial_coefficient) counting the ways of choosing an (unordered) subset of _k_ elements from a fixed set of _n_ elements, to check that 
$$
\frac{\mathrm{d}f}{dx}=n\,x^{n-1}
$$
for $f(x)=x^{n}$ and all $n>0$ in $\mathbb{N}$.

---

2) Compute the derivative of $([0,+\infty),\mathbb{R},f,\mathbb{R})$, where $f(x)=\sqrt[n]{x}=x^{\frac{1}{n}}$ with $n>1$, at each point.


>[!note]- Solution
>A direct computation shows that $([0,+\infty),\mathbb{R},f,\mathbb{R})$ is the inverse function of $([0,+\infty),\mathbb{R},g,\mathbb{R})$ with $g(y)=y^{n}$. The function $([0,+\infty),\mathbb{R},g,\mathbb{R})$ is differentiable for every $y>0$. Therefore, [[1.3 Derivatives of scalar functions#^05d051\|we conclude that]] $([0,+\infty),\mathbb{R},f,\mathbb{R})$ is differentiable for each $x>0$, and its derivative reads
>$$ f'(x)=\frac{1}{n} x^{\frac{1}{n}-1}.$$
>At $y=0$, we can only compute the right derivative of $([0,+\infty),\mathbb{R},g,\mathbb{R})$ . It turns out this derivative vanishes, and thus $([0,+\infty),\mathbb{R},f,\mathbb{R})$ has no right derivative at $x=0$.

---

3) Determine for which $x\in\mathbb{R}$ the function $(\mathbb{R},\mathbb{R},f,\mathbb{R})$ is differentiable in the following cases:
	$$ \begin{split}
	1) \quad & f(x)= |x - 2| \\ & \\
	2) \quad & f(x)= \sqrt{|x|} \\ & \\
	3) \quad & f(x)= \left\{\begin{matrix}  x^{2} & \mbox{ if } x\leq 1 \\ 2-x & \mbox{ if } x> 1\end{matrix}\right. \\ & \\
	4) \quad & f(x)= \left\{\begin{matrix} x^{2} -1 & \mbox{ if } x\leq 2 \\  3 & \mbox{ if } x> 2\end{matrix}\right. \\ & \\
	5)\quad & f(x)= \left\{\begin{matrix}  4x & \mbox{ if } x<1 \\ 2x +2 & \mbox{ if } x\geq 1\end{matrix}\right. \\ & \\
	1) \quad & f(x)= \left\{\begin{matrix}  \frac{-x^{2}}{2}  & \mbox{ if } x<3 \\ -3x & \mbox{ if } x\geq 3\end{matrix}\right. \end{split} $$


>[!note]- Solution
>1) Given the appearance of the absolute value, we split our function in two pieces: $([2,\infty),\mathbb{R},f_{1},\mathbb{R})$ with $f_{1}(x)=x-2=f(x)$, and $((-\infty,2],\mathbb{R},f,\mathbb{R})$, with $f_{2}(x)=2-x=f(x)$. Since we already know the derivative of constant and linear functions, and since we have  behave  Note that the function $((2,\infty),\mathbb{R},f_{1},\mathbb{R})$, with $f_{1}(x)=x-2=f(x)$, the [[1.3 Derivatives of scalar functions#^5d20ad\|algebraic manipulations of derivatives]] ensure $([2,\infty),\mathbb{R},f_{1},\mathbb{R})$ is differentiable for every $x>2$, and its right derivative at $x=2$ is equal to 1. Proceeding analogously for $((-\infty,2],\mathbb{R},f,\mathbb{R})$, with $f_{2}(x)=2-x=f(x)$, we obtain it is differentiable for every $x<2$, and its left derivative at $x=2$ is $-1$. We thus conclude that $(\mathbb{R},\mathbb{R},f,\mathbb{R})$ is differentiable everywhere except at $x=2$.
>2) Following the idea used in point 1), we split the function in two pieces: $([0,\infty),\mathbb{R},f_{1},\mathbb{R})$ with $f_{1}(x)=\sqrt{x}=f(x)$, and $((-\infty,0],\mathbb{R},f,\mathbb{R})$, with $f_{2}(x)=\sqrt{-x}=f(x)$. 
>3) Following the idea used in point 1) we conclude the function is differentiable for every $x\neq 1$.
>4) Following the idea used in point 1) we conclude the function is differentiable for every $x\neq 2$.
>5) Following the idea used in point 1) we conclude the function is differentiable for every $x\neq 1$.
>6) Following the idea used in point 1) we conclude the function is differentiable everywhere.

---

4) Whenever possible, compute the derivatives at all points in the maximal domain of the scalar functions determined by:

$$
\begin{split}
1) \quad &  f(x)= x^{\frac{m}{n}}  \\  & \\
2) \quad &  f(x)= \frac{2x}{1-x}  \\  & \\
3) \quad &  f(x)=\frac{x}{1-x}\,\frac{2-x}{3+x}  \\  & \\
4) \quad &  f(x)=\frac{(x^{2} +1)^{3}}{x+3}   \\  & \\
5) \quad &  f(x)=\sqrt{x^{4} + 3x^{2} -2}  \\  & \\
6) \quad &  f(x)=\sqrt{\frac{x +2}{x^{2}}}  \\  & \\
7) \quad &  f(x)=\frac{x}{\sqrt{x+2}}  \\  & \\
8) \quad &    f(x)=(g(x))^{\frac{m}{n}}
\end{split}
$$


>[!note]- Solution
>1) The maximal domain is $[0,+\infty)$. Using the result of exercise 2.2) above together with the [[1.3 Derivatives of scalar functions#^c87d27\|chain rule]], we obtain
>$$ f'(x)=\frac{m}{n}x^{\frac{m}{n}-1}$$
>for every $x>0$, and the right derivative at $x=0$ is $0$ when $m\geq n$, and undefined when $m<n$.
>2) The maximal domain is $(-\infty,1)\cup (1,+\infty)$. Using the [[1.3 Derivatives of scalar functions#^5d20ad\|algebraic manipulation of derivatives]] we obtain
>$$f'(x)=\frac{2}{(1-x)^{2}}.$$
>3) The maximal domain is $(-\infty,-3)\cup(-3,1)\cup(1,+\infty)$. The derivative is then computed using the [[1.3 Derivatives of scalar functions#^5d20ad\|algebraic manipulation of derivatives]]. You can check your result [here](https://onsolver.com/ ), or look in the [[Home#Tools to help with exercises\|home]] for further suggestions.
>4) The maximal domain is $(-\infty,-3)\cup(-3,+\infty)$. The derivative is then computed using the [[1.3 Derivatives of scalar functions#^5d20ad\|algebraic manipulation of derivatives]]. You can check your result [here](https://onsolver.com/ ), or look in the [[Home#Tools to help with exercises\|home]] for further suggestions.
>5) The maximal domain is the subset on which $x^{4}+3x^{2}-2\geq 0$. The derivative is then computed using the [[1.3 Derivatives of scalar functions#^5d20ad\|algebraic manipulation of derivatives]]. You can check your result [here](https://onsolver.com/ ), or look in the [[Home#Tools to help with exercises\|home]] for further suggestions.
>6) The maximal domain is $[-2,0)\cup(0,+\infty)$. The right derivative at $x=-2$ does not exist, while the derivative in the other points is computed using the [[1.3 Derivatives of scalar functions#^5d20ad\|algebraic manipulation of derivatives]]. You can check your result [here](https://onsolver.com/ ), or look in the [[Home#Tools to help with exercises\|home]] for further suggestions.
>7) The maximal domain is $(-2,+\infty)$. The derivative is then computed using the [[1.3 Derivatives of scalar functions#^5d20ad\|algebraic manipulation of derivatives]]. You can check your result [here](https://onsolver.com/ ), or look in the [[Home#Tools to help with exercises\|home]] for further suggestions.
>8) The maximal domain here is the subset on which $g(x)\geq 0$. Then, we can use the [[1.3 Derivatives of scalar functions#^c87d27\|chain rule]] to get
>$$ f'(x)=\frac{m}{n}(g(x))^{\frac{m}{n}-1}\,g'(x)$$
>at all those $x$ at which $g$ is differentiable and such that $g(x)>0$. When $g$ is differentiable but $g(x)=0$, the right derivative is undefined when $m<n$ and equal to $0$ when $m\geq n$. Obviously, at all those points at which $g$ is not differentiable, then $f$ is not differentiable.




# 3 Numerical sequences and series



1) Prove the following limits 
	$$ \begin{split} 
	1) \quad & \lim_{n\rightarrow+\infty}\, n!= + \infty \\ & \\
	2) \quad &  \lim_{n\rightarrow+\infty}\,\frac{x^{n}}{n!}=0\quad\mbox{ for }\quad |x|\leq 1    \\ & \\
	3) \quad &  \lim_{n\rightarrow +\infty}\,\sqrt[n]{n}=1  \\ & \\
	4) \quad & \lim_{n\rightarrow + \infty}\, \sqrt[n]{n!} = +\infty  \\ & \\
	5) \quad & \lim_{n\rightarrow +\infty}\,kx^{k+2}-(k+1)x^{k+1}=\left\{\begin{matrix}0 &\mbox{ if } |x|<1 \\ +\infty & \mbox{ if } x>1 \\ \nexists & \mbox{ if } x<-1\end{matrix}\right.     \end{split} $$
	>[!note]- Solution
	>1) Because of the factorial, we can not rely on limits of functions. We must prove that, for every $K>0$, there exists $N\in\mathbb{N}$ such that $a_{n}=n!>K$ for all $n>N$. When $n>1$, it holds $n!=n(n-1)\cdots 1> n$, so that, setting $n=N>K$, we get $a_{n}=n!>n>K$ as desired.
	>2) For $|x|\leq 1$, the sequence $a_{n}=x^{n}$ has limit either $0$ or $1$ (only when $x=\pm1$). Therefore, exploiting the result of point 1) together with the algebraic manipulations of limits of sequences, the desired result follows.   
	>3) Set $b_{n}\equiv \sqrt[n]{n} -1>0$, so that $n=(1+b_{n})^{n}$. Recalling [Newton's binomial formula](https://en.wikipedia.org/wiki/Binomial_theorem)
	>	$$ (a+b)^{n}=\sum\limits_{k=0}^{n}{n\choose k} a^{n-k}b^{k}=\sum\limits_{k=0}^{n}{n\choose k} a^{k}b^{n-k}, $$ 
	>	it follows that 
	>	$$ n=(1+b_{n})^{n}=\sum\limits_{k=0}^{n}{n\choose k} 1^{k}b_{n}^{n-k}\,\stackrel{k=n-2}{\geq}\, \frac{n(n-1)}{2!}b_{n}^{2}, $$ 
	>	which means that $0\leq b_{n}\leq\sqrt{\frac{2}{(n-1)}}$. The squeeze theorem for sequences then implies 
	>	$$ \lim_{n\rightarrow+\infty} b_{n}=0\;\Longleftrightarrow\; \lim_{n\rightarrow+\infty} \sqrt[n]{n}-1=0 ,$$ 
	>	which proves the desired equality.
	>4) Since $n!=n(n-1)\cdots 2\cdot 1)$,  it holds $n!\geq (\sqrt{\frac{n}{2}})^{n}$ (just take the quotient of the two quantities and expand them es products of terms). Therefore, $\sqrt[n]{n!}\geq \sqrt{\frac{n}{2}}$, and the result follows taking $N>2K^{2}$ in the definition of [[1.4 Sequences and series#^5a7f61\|unbounded limit]].
	>5) dds
	---
  
{ #98a973}

2) Compute the value of the truncated geometric series associated with 
	$$ a_{n} = \left\{ \begin{matrix} a_{n}=0 & \mbox{ for } n=0,...,r-1 \\ a_{n} = x^{n} & \mbox{ for } n\geq r . \end{matrix} \right. $$
	>[!note]- Solution
	>The trick is to realize that  
	>$$ \sum_{n=0}^{+\infty}a_{n}=\sum_{n=r}^{+\infty}x^{n}= \sum_{n=0}^{+\infty}x^{n+r} = x^{r}\sum_{n=0}^{+\infty}x^{n}, $$
	>which means that the truncated geometric series is proportional to the [[1.4 Sequences and series#^bf33d9\|geometric series]], and thus its convergence, as well as its sum, can be deduced from the geometric series.
	---
3) Determine the behavior of the arithmetic-geometric series defined by $a_{n}=nx^{n}$ (starting at $n=0$ or $n=1$).
	>[!note]- Solution
	>First of all, starting at $n=0$ or $n=1$ is irrelevant for the result. Then, once again, the series diverges when $x=1$ because
	>$$ S_{k}=\sum\limits_{n=0}^{k}a_{n}=1+2+3+\cdots+(k-1) + k \frac{k(k+1)}{2}$$.
	>When $k\neq 1$, we have
	>$$ S_{k}-xS_{k}=(x+2x^{2}+3x^{3}+\cdots+kx^{k})-(x^{2}+2x^{3}+3x^{4}+kx^{k+1})=x+x^{2}+\cdots +x^{k} -kx^{k+1}$$. 
	>The positive terms in the right-hand-side from the partial sum of the [[1.4 Sequences and series#^bf33d9\|geometric series]] apart from the first term. Therefore, we have
	>$$ (1-x)S_{k}=\frac{x^{k+1}-1}{x-1} -1 -kx^{k+1}=\frac{x-(k+1)x^{k+1} +kx^{k+2}}{1-x}  \Longrightarrow S_{k}=\frac{x-(k+1)x^{k+1} +kx^{k+2}}{(1-x)^{2}} .$$
	>Because of exercise 3.1.5), when $x>1$ the sequence of partial sums diverges, when $x<-1$ it does not have a limit, while it converges to $0$ when $|x|<1$. Consequently, the sum of the arithmetic-geometric series is 
	>$$ \sum\limits_{n=0}^{+\infty}nx^{n}=\frac{x}{(1-x)^{2}} $$
	>when $|x|<1$, while its either unbounded or undefined in the other cases.
	---
4) Prove that, if $a_{n}=u_{n}-u_{n+1}$ for some sequence $\{u_{n}\}_{n\in\mathbb{N}}$ (**telescoping series**), then 
	$$ \sum\limits_{n=1}^{\infty}a_{n}=u_{1}-\lim_{n\rightarrow\infty}u_{n} .$$
	>[!note]- Solution
	>The partial sum of the series determined by $a_{n}$ reads 
	>$$ S_{k}=\sum\limits_{n=1}^{k}u_{n}-u_{n+1}=u_{1}-u_{k+1}, $$
	>and the result follows from the [[1.4 Sequences and series#^32251b\|very definition]] of the sum of a series.
	---
5) Check the following equalities: 
	$$ \begin{split}
	1) &\qquad  \sum_{n=1}^{+\infty}\,\frac{1}{2n(n+1)}\,=\;\frac{1}{2}\\ & \\
	2)  &\qquad  \sum_{n=0}^{+\infty}\;\frac{n}{10^{n}} \,=\;\frac{10}{81} \\ & \\
	3)  &\qquad   \sum_{n=2}^{+\infty}\;\frac{1}{n^{2} -n}\,=\;1 \\ & \\
	4)  &\qquad  \sum_{n=0}^{+\infty}\;\frac{1}{(n+1)(n+3)} \,=\; \frac{3}{4}\\ & \\
	5)  &\qquad  \sum_{n=0}^{+\infty}\;\frac{2^{n+3}}{3^{n}}\,=\;.\end{split}$$
	>[!note]- Solution
	>1) The result follows from exercise 3.4) above once we note that $a_{n}=\frac{1}{2}(\frac{1}{n}-\frac{1}{n+1})$.
	>2) This exercise deserves no solution.
	>3) We note that $a_{n}= \frac{1}{n-1}-\frac{1}{n}$. Then, we perform the replacement $n=k+1$ so that 
	>	$$ \sum\limits_{n=2}^{+\infty}a_{n}\rightarrow\sum\limits_{k=1}^{+\infty}a_{k} $$
	>	with $a_{k}=\frac{1}{k}-\frac{1}{k+1}$, and the result follows again from exercise 3.4) above. 
	>4) We note that $a_{n}=\frac{1}{2}(\frac{1}{n+1} - \frac{1}{n+3})$, so that the replacement $k=n+1$ gives $a_{k}=\frac{1}{2}(\frac{1}{k} - \frac{1}{k+2})$. Now, we can not directly use the result of exercise 3.4) above, however, we can adapt the proof used there to this case and obtain
	>	$$\sum\limits_{k=1}^{\infty}a_{k}=\sum\limits_{k=1}u_{k}-u_{k+2}=u_{1}+u_{2}+\lim_{k\rightarrow+\infty}u_{k} $$,
	>	from which the desired result immediately follows.
	>5) 
	---




# 4 Power series and Taylor expansion 



1) Compute the Taylor expansion of the following functions: 


>[!note]- Solution




# 5 Limits and derivatives of trascendental functions



1) Whenever possible, compute the derivatives at all points in the maximal domain of the scalar functions determined by:

$$
\begin{split} 
1) \quad &  f(x) =\ln(x) \\ & \\ 
2) \quad & f(x) =\ln(|x|) \\ & \\
3) \quad & f(x)= x^{\alpha}   \\ & \\
4) \quad & f(x) = \arcsin(x) \\ & \\
5) \quad & f(x) = \arccos(x) \\ & \\
6) \quad & f(x) = \tan(x)  \\ & \\
7) \quad & f(x) =\cot(x) \\ & \\
8) \quad & f(x) = \arctan(x) \\ & \\
9) \quad & f(x) =  x^{x} \\ & \\
10) \quad & f(x) = \sqrt{\tan(x)} \\ & \\
11) \quad & f(x) = \arctan\left(x^{3} - e^{x^{2}}\right) \\ & \\
12) \quad &  f(x)=(g(x))^{h(x)} \\ & \\
13) \quad & f(x)= \arctan\left(\frac{g(x)}{h(x)}\right)
\end{split}
$$


>[!note]- Solution

---

3) 
$$
\begin{split}
\quad & \lim_{n\rightarrow+\infty}\,x^{\frac{1}{n}}=1 \quad\mbox{ for all }\quad x>0 \\ & \\
3) \quad & \lim_{n\rightarrow+\infty}\,x^{n}=0\quad\mbox{ for all }\quad |x|<1     \\ & \\
4) \quad & \lim_{n\rightarrow+\infty}\,n^{-\alpha}=0\quad\mbox{ for all }\quad \alpha>0    \\ & \\
\end{split}
$$

1) Use L'Hôpital's rule or Taylor's approximation to check the following limits:

$$
\begin{split} 
1) \quad & \lim_{x\rightarrow 0}\, \frac{\sin(x)}{x}= 1\\ & \\
2) \quad & \lim_{x\rightarrow 0}\,\frac{\mathrm{e}^{x} - x - \cos(x)}{\sin(x^{2})} =  \\ & \\
3) \quad & \lim_{x\rightarrow +\infty}\,\left(1 + \frac{1}{x}\right)^{x}=  \\ & \\
4) \quad & \lim_{x\rightarrow +\infty}\, \frac{\left(1 + \frac{1}{x}\right)^{x^{2}}}{\mathrm{e}^{x}} = \\ & \\
5) \quad & \lim_{x\rightarrow + \infty} \frac{\ln(x)}{x^{\alpha}} =
\end{split}
$$


>[!note]- Solution
